src/ByteString.v
@@ -1,7 +1,8 @@
 Require Import
   Fiat.ADT
   Fiat.ADTNotation
-  ByteString.Memory.
+  ByteString.Memory
+  Hask.Control.Applicative.
 
 (************************************************************************
  ** Semantics of the core Haskell ByteString data type in Fiat.        **
@@ -13,17 +14,23 @@ Definition emptyS  := "empty".
 Definition consS   := "cons".
 Definition unconsS := "uncons".
 
+Section ByteString.
+
+Context `{Alternative m}.
+
 Definition ByteStringSpec := Def ADT {
   rep := list Word,
 
   Def Constructor0 emptyS : rep := ret []%list,,
 
-  Def Method1 consS (r : rep) (w : Word) : rep * unit :=
-    ret (cons w r, tt),
-  Def Method0 unconsS (r : rep) : rep * (option Word) :=
+  Def Method1 consS (r : rep) (w : Word) : rep * m unit :=
+    u <- { u : m unit | True };
+    ret (cons w r, u),
+  Def Method0 unconsS (r : rep) : rep * m (option Word) :=
+    u <- { u : m unit | True };
     ret (match r with
-         | nil => (r, None)
-         | cons x xs => (xs, Some x)
+         | nil => (r, u *> pure None)
+         | cons x xs => (xs, u *> pure (Some x))
          end)
 
 }%ADTParsing.
@@ -33,8 +40,10 @@ Definition ByteString := Rep ByteStringSpec.
 Definition empty : Comp ByteString :=
   Eval simpl in callCons ByteStringSpec emptyS.
 
-Definition cons (w : Word) (bs : ByteString) : Comp ByteString :=
-  Eval simpl in (p <- callMeth ByteStringSpec consS bs w; ret (fst p)).
+Definition cons (w : Word) (bs : ByteString) : Comp (ByteString * m unit) :=
+  Eval simpl in callMeth ByteStringSpec consS bs w.
 
-Definition uncons (bs : ByteString) : Comp (ByteString * option Word) :=
+Definition uncons (bs : ByteString) : Comp (ByteString * m (option Word)) :=
   Eval simpl in callMeth ByteStringSpec unconsS bs.
+
+End ByteString.
