src/ByteStringHeap.v
@@ -7,7 +7,9 @@ Require Import
   ByteString.HeapCanon
   ByteString.ByteString
   Coq.FSets.FMapFacts
-  Coq.Structures.DecidableTypeEx.
+  Coq.Structures.DecidableTypeEx
+  Hask.Control.Applicative
+  Hask.Control.Monad.
 
 Module ByteStringHeap (M : WSfun N_as_DT).
 
@@ -19,8 +21,30 @@ Import FMapExt.
 
 Open Scope N_scope.
 
-Record PS := makePS {
-  psHeap : Rep HeapSpec;
+Class Computable (m : Type -> Type) := {
+  (* Parametricity gives us the only laws we should need. Note that this can
+     allow for multiple interpretations: for the list monad, we might choose
+     computation to mean that any member in the list has the given value, or
+     that only the first or last one does, etc. *)
+  m_computes_to {A : Type} (ca : m A) (a : A) : Prop
+}.
+
+Notation "'Ifcomputes' x 'as' v 'Then' t 'Else' e" :=
+  (mv <- { mv | forall v, IF m_computes_to x v
+                          then mv = Some v
+                          else mv = None };
+   Ifopt mv as v
+   Then t
+   Else e)%comp (at level 100).
+
+Section ByteStringHeap.
+
+Context `{Monad m}.
+Context `{Alternative m}.
+Context `{Computable m}.
+
+Record PS (heapType : Type) := makePS {
+  psHeap : heapType;
 
   psBuffer : Ptr;
   psBufLen : Size;
@@ -29,89 +53,108 @@ Record PS := makePS {
   psLength : Size
 }.
 
-Definition simply_widen_region (r : PS) : PS :=
+Definition PSH := PS (Rep HeapSpec).
+
+Definition simply_widen_region (r : PSH) : PSH :=
   {| psHeap   := psHeap r
    ; psBuffer := psBuffer r
    ; psBufLen := psBufLen r
    ; psOffset := psOffset r - 1
    ; psLength := psLength r + 1 |}.
 
-Program Definition make_room_by_shifting_up (r : PS) (n : N | 0 < n) :
+Program Definition make_room_by_shifting_up (r : PSH) (n : N | 0 < n) :
   (* We could maybe be smarter by shifting the block so it sits mid-way within
      the buffer. *)
-  Comp PS :=
-  res <- memcpy (psHeap r) (psBuffer r) (psBuffer r + n) (psLength r);
-  ret {| psHeap   := fst res
-       ; psBuffer := psBuffer r
-       ; psBufLen := psBufLen r
-       ; psOffset := 0
-       ; psLength := psLength r + n |}.
+  Comp (PSH * m unit) :=
+  `(h, mres) <- memcpy (psHeap r) (psBuffer r) (psBuffer r + n) (psLength r);
+  Ifcomputes mres as u
+  Then ret ({| psHeap   := h
+             ; psBuffer := psBuffer r
+             ; psBufLen := psBufLen r
+             ; psOffset := 0
+             ; psLength := psLength r + n |}, pure u)
+  Else ret (r, mres).
 
-Program Definition make_room_by_growing_buffer (r : PS) (n : N | 0 < n) :
-  Comp PS :=
+Program Definition make_room_by_growing_buffer (r : PSH) (n : N | 0 < n) :
+  Comp (PSH * m unit) :=
   (* We can make a trade-off here by allocating extra bytes in anticipation of
      future calls to [buffer_cons]. *)
-  `(h, a) <- alloc (psHeap r) (psLength r + n);
-  `(h, _) <- memcpy h (psBuffer r) (a + n) (psLength r);
-  `(h, _) <- free h (psBuffer r);
-  ret {| psHeap   := h
-       ; psBuffer := a
-       ; psBufLen := psLength r + n
-       ; psOffset := 0
-       ; psLength := psLength r + n |}.
+  `(h, ma) <- alloc (psHeap r) (psLength r + n);
+  Ifcomputes ma as a
+  Then (
+    `(h, mres) <- memcpy h (psBuffer r) (a + n) (psLength r);
+    Ifcomputes mres as u
+    Then (
+      `(h, mres) <- free h (psBuffer r);
+      Ifcomputes mres as u
+      Then ret ({| psHeap   := h
+                 ; psBuffer := a
+                 ; psBufLen := psLength r + n
+                 ; psOffset := 0
+                 ; psLength := psLength r + n |}, pure u)
+      Else ret (r, mres)
+    )
+    Else ret (r, mres)
+  )
+  Else ret (r, fmap (const tt) ma).
 Obligation 1. nomega. Defined.
 
 Program Definition allocate_buffer (r : Rep HeapSpec) (len : N | 0 < len) :
-  Comp PS :=
-  `(h, a) <- alloc r len;
-  ret {| psHeap   := h
-       ; psBuffer := a
-       ; psBufLen := len
-       ; psOffset := 0
-       ; psLength := len |}.
+  Comp (PSH * m unit) :=
+  `(h, ma) <- alloc r len;
+  Ifcomputes ma as a
+  Then ret ({| psHeap   := h
+             ; psBuffer := a
+             ; psBufLen := len
+             ; psOffset := 0
+             ; psLength := len |}, pure tt)
+  Else ret (makePS r 0 0 0 0, fmap (const tt) ma).
 
-Definition poke_at_offset (r : PS) (d : Word) : Comp PS :=
-  res <- poke (psHeap r) (psBuffer r + psOffset r) d;
-  ret {| psHeap   := fst res
-       ; psBuffer := psBuffer r
-       ; psBufLen := psBufLen r
-       ; psOffset := psOffset r
-       ; psLength := psLength r |}.
+Definition poke_at_offset (r : PSH) (d : Word) : Comp (PSH * m unit) :=
+  `(h, mres) <- poke (psHeap r) (psBuffer r + psOffset r) d;
+  Ifcomputes mres as u
+  Then ret ({| psHeap   := h
+             ; psBuffer := psBuffer r
+             ; psBufLen := psBufLen r
+             ; psOffset := psOffset r
+             ; psLength := psLength r |}, pure u)
+  Else ret (r, mres).
 
 (* This defines how much a buffer is grown by when more space is needed to
    [cons] on a new element. *)
 Definition alloc_quantum := 1.
 Arguments alloc_quantum /.
 
-Program Definition buffer_cons (r : PS) (d : Word) : Comp PS :=
-  ps <- If 0 <? psOffset r
-        Then ret (simply_widen_region r)
-        Else
-        If psLength r + alloc_quantum <=? psBufLen r
-        Then make_room_by_shifting_up r alloc_quantum
-        Else
-        If 0 <? psBufLen r
-        Then make_room_by_growing_buffer r alloc_quantum
-        Else allocate_buffer (psHeap r) alloc_quantum;
-  poke_at_offset ps d.
+Program Definition buffer_cons (r : PSH) (d : Word) : Comp (PSH * m unit) :=
+  `(ps, mres) <-
+     If 0 <? psOffset r
+     Then ret (simply_widen_region r, pure tt)
+     Else If psLength r + alloc_quantum <=? psBufLen r
+          Then make_room_by_shifting_up r alloc_quantum
+          Else If 0 <? psBufLen r
+               Then make_room_by_growing_buffer r alloc_quantum
+               Else allocate_buffer (psHeap r) alloc_quantum;
+  Ifcomputes mres as u
+  Then poke_at_offset ps d
+  Else ret (r, mres).
 Obligation 1. nomega. Defined.
 Obligation 2. nomega. Defined.
 Obligation 3. nomega. Defined.
 
-Definition buffer_uncons (r : PS) : Comp (PS * option Word) :=
+Definition buffer_uncons (r : PSH) : Comp (PSH * m (option Word)) :=
   If 0 <? psLength r
   Then (
-    w <- peek (psHeap r) (psBuffer r + psOffset r);
+    `(r', mw) <- peek (psHeap r) (psBuffer r + psOffset r);
     ret ({| psHeap   := psHeap r
           ; psBuffer := psBuffer r
           ; psBufLen := psBufLen r
           ; psOffset := if psLength r =? 1
                         then 0
                         else psOffset r + 1
-          ; psLength := psLength r - 1 |}, Some (snd w)))
-  Else ret (r, None).
+          ; psLength := psLength r - 1 |}, fmap Some mw))
+  Else ret (r, pure None).
 
-Definition ByteString_list_AbsR (or : Rep ByteStringSpec) (nr : PS) :=
+Definition ByteString_list_AbsR (or : Rep ByteStringSpec) (nr : PSH) :=
   length or = N.to_nat (psLength nr) /\
   IF psBufLen nr = 0
   then psOffset nr = 0 /\ psLength nr = 0
@@ -135,48 +178,76 @@ Ltac destruct_AbsR H :=
 
 Ltac construct_AbsR := split; try split; simpl; try nomega.
 
+Local Ltac breakdown :=
+  repeat (
+    destruct_computations; simpl in *;
+    computes_to_inv; try tsubst; simpl in *;
+    match goal with
+      [ H : option _ |- _ ] => destruct H; simpl in *
+    end;
+    computes_to_inv; try tsubst; simpl in *).
+
 Lemma buffer_cons_sound : forall r_o r_n,
   ByteString_list_AbsR r_o r_n
-    -> forall x r_n', buffer_cons r_n x ↝ r_n'
+    -> forall x r_n' mu, buffer_cons r_n x ↝ (r_n', mu)
+    -> forall u, m_computes_to mu u
     -> ByteString_list_AbsR (x :: r_o) r_n'.
 Proof.
-  unfold buffer_cons; intros ? ? AbsR ???.
-  apply refine_computes_to in H.
-  rewrite refineEquiv_If_Then_Else_Bind in H.
-  apply refine_If_Then_Else_bool in H.
+  unfold buffer_cons; intros ? ? AbsR ??????.
+  apply refine_computes_to in H2.
+  unfold Bind2 in H2.
+  rewrite refineEquiv_If_Then_Else_Bind in H2.
+  apply refine_If_Then_Else_bool in H2.
   destruct (0 <? psOffset r_n) eqn:Heqe.
-    apply computes_to_refine in H.
+    apply computes_to_refine in H2.
     {
-      destruct_computations; simpl in *.
       destruct_AbsR AbsR; construct_AbsR.
-      right; split; trivial; split; [nomega|].
+        breakdown; try nomega.
+        destruct u, (H8 tt); intuition.
+        discriminate.
+      right; split.
+        breakdown; nomega.
+      split; intros; simpl.
+        breakdown; nomega.
       split; intros.
-        simpl; trivial.
-      simplify_maps.
-      destruct i using N.peano_ind.
-        left; nomega.
-      right; split; [nomega|].
-      rewrite <- N.add_assoc.
-      rewrite <- N.add_sub_swap; [|nomega].
-      rewrite <- N.add_sub_assoc; [|nomega].
-      rewrite N.add_assoc.
-      apply H4; [nomega|].
-      rewrite N2Nat.inj_sub.
-      replace (N.to_nat 1) with 1%nat; [|nomega].
-      simpl; rewrite N2Nat.inj_succ in *; simpl.
-      rewrite Nat.sub_0_r; assumption.
+        breakdown; nomega.
+      breakdown.
+      - inversion H13; simpl in *; clear H13.
+        revert H9.
+        subst; simpl in *; intros.
+        simplify_maps.
+        destruct i using N.peano_ind.
+          left; nomega.
+        right; split; [nomega|].
+        rewrite <- N.add_assoc.
+        rewrite <- N.add_sub_swap; [|nomega].
+        rewrite <- N.add_sub_assoc; [|nomega].
+        rewrite N.add_assoc.
+        apply H7; [nomega|].
+        rewrite N2Nat.inj_sub.
+        replace (N.to_nat 1) with 1%nat; [|nomega].
+        simpl; rewrite N2Nat.inj_succ in *; simpl.
+        rewrite Nat.sub_0_r; assumption.
+      - admit.
+      - admit.
+      - admit.
+      - admit.
     }
   assert (psOffset r_n = 0) by nomega; clear Heqe.
-  rewrite refineEquiv_If_Then_Else_Bind in H.
-  apply refine_If_Then_Else_bool in H.
+  rewrite refineEquiv_If_Then_Else_Bind in H2.
+  apply refine_If_Then_Else_bool in H2.
   destruct (psLength r_n + alloc_quantum <=? psBufLen r_n) eqn:Heqe2;
-  [| rewrite refineEquiv_If_Then_Else_Bind in H;
-     destruct (0 <? psBufLen r_n) eqn:Heqe3; simpl in H ];
-  apply computes_to_refine in H; revert H;
+  [| rewrite refineEquiv_If_Then_Else_Bind in H2;
+     destruct (0 <? psBufLen r_n) eqn:Heqe3; simpl in H2 ];
+  apply computes_to_refine in H2; revert H2;
   unfold make_room_by_shifting_up, make_room_by_growing_buffer,
          allocate_buffer, poke_at_offset;
   autorewrite with monad laws; simpl;
   rewrite ?N.add_0_r.
+  admit.
+  admit.
+  admit.
+(*
   - simpl; intros; destruct_computations;
     destruct_AbsR AbsR; construct_AbsR;
     (right; split; [nomega|]; split; [nomega|]).
@@ -242,24 +313,29 @@ Proof.
       left; nomega.
     right; split; [nomega|].
     rewrite N2Nat.inj_succ in *; nomega.
-Qed.
+*)
+Admitted.
 
 Lemma buffer_uncons_sound : forall r_o r_n a,
   ByteString_list_AbsR r_o r_n
-    -> buffer_uncons r_n ↝ a
+    -> forall mp, buffer_uncons r_n ↝ (a, mp)
+    -> forall p, m_computes_to mp p
     -> ByteString_list_AbsR (match r_o with
                              | [] => r_o
                              | _ :: xs => xs
-                             end) (fst a).
+                             end) a.
 Proof.
   unfold buffer_uncons; intros.
-  apply refine_computes_to in H0.
-  apply refine_If_Then_Else_bool in H0.
+  apply refine_computes_to in H3.
+  apply refine_If_Then_Else_bool in H3.
   destruct (0 <? psLength r_n) eqn:Heqe.
-    revert H0.
-    autorewrite with monad laws; simpl; intros.
-    apply computes_to_refine in H0.
+    revert H3.
+    unfold peek, Bind2, conditionally.
+    rewrite refineEquiv_bind_bind; intros.
+    apply computes_to_refine in H3.
     destruct_computations; simpl.
+    admit.
+(*
     destruct_AbsR H; construct_AbsR;
     destruct x; try destruct p; simpl in *;
     destruct r_o; simpl in *;
@@ -280,30 +356,37 @@ Proof.
     rewrite N.add_succ_l.
     rewrite N2Nat.inj_succ in *; simpl.
     rewrite N2Nat.inj_add, Nat.add_1_r; trivial.
-  apply computes_to_refine in H0.
-  destruct_computations.
+*)
+  apply computes_to_refine in H3.
+(*
+  breakdown.
   destruct_AbsR H; construct_AbsR;
   destruct r_o; simpl in *; auto; try nomega.
     left; intuition.
   right; intuition.
-Qed.
+*)
+Admitted.
 
 Lemma buffer_uncons_impl : forall r_o r_n a,
   ByteString_list_AbsR r_o r_n
-    -> buffer_uncons r_n ↝ a
-    -> snd a = match r_o with
+    -> forall mp, buffer_uncons r_n ↝ (a, mp)
+    -> forall p, m_computes_to mp p
+    -> p = match r_o with
                | [] => None
                | x :: _ => Some x
                end.
 Proof.
   unfold buffer_uncons; intros.
-  apply refine_computes_to in H0.
-  apply refine_If_Then_Else_bool in H0.
+  apply refine_computes_to in H3.
+  apply refine_If_Then_Else_bool in H3.
   destruct (0 <? psLength r_n) eqn:Heqe.
-    revert H0.
-    autorewrite with monad laws; simpl; intros.
-    apply computes_to_refine in H0.
+    revert H3.
+    unfold peek, Bind2, conditionally.
+    rewrite refineEquiv_bind_bind; intros.
+    apply computes_to_refine in H3.
     destruct_computations.
+    admit.
+(*
     destruct_AbsR H; simpl;
     destruct r_o; simpl in *; try nomega.
     f_equal; tsubst.
@@ -312,16 +395,19 @@ Proof.
        with (psBuffer r_n + psOffset r_n + 0) by nomega.
     apply H4; trivial.
     nomega.
-  apply computes_to_refine in H0.
-  apply Return_inv in H0.
+*)
+  apply computes_to_refine in H3.
+  apply Return_inv in H3.
   destruct a; tsubst; simpl in *.
+(*
   destruct r_o; simpl in *;
-  destruct H, H0; auto.
+  destruct H, H0; auto
     destruct H0, H1.
     rewrite H2 in H; simpl in H.
     discriminate.
   nomega.
-Qed.
+*)
+Admitted.
 
 Theorem ByteStringHeap (heap : Rep HeapSpec) :
   { adt : _ & refineADT ByteStringSpec adt }.
@@ -347,10 +433,16 @@ Proof.
       eapply (refine_skip2 (dummy:=buffer_cons r_n d)).
     etransitivity.
       apply refine_under_bind; intros; simpl.
-      refine pick val a.
+
+      destruct a.
+      refine pick val m0; auto.
+      simplify with monad laws; simpl.
+
+      refine pick val p.
         simplify with monad laws.
         finish honing.
-      eapply buffer_cons_sound; eauto.
+      admit.
+      (* eapply buffer_cons_sound; eauto. *)
     simplify with monad laws; simpl.
     finish honing.
   }
@@ -361,19 +453,27 @@ Proof.
       eapply (refine_skip2 (dummy:=buffer_uncons r_n)).
     etransitivity.
       apply refine_under_bind; intros; simpl.
-      pose proof H1.
-      eapply buffer_uncons_impl in H1; eauto.
-      rewrite fst_match_list, snd_match_list, <- H1.
-      refine pick val (fst a).
+      destruct a.
+      refine pick val (fmap (const tt) m0); auto.
         simplify with monad laws.
-        rewrite <- surjective_pairing.
-        finish honing.
-      eapply buffer_uncons_sound; eauto.
+        pose proof H4.
+        eapply buffer_uncons_impl in H4; eauto.
+        (* rewrite fst_match_list, snd_match_list, <- H4. *)
+        refine pick val p.
+          simplify with monad laws.
+          (* rewrite <- surjective_pairing. *)
+          (* finish honing. *)
+          admit.
+        (* eapply buffer_uncons_sound; eauto. *)
+        admit.
+      admit.
     simplify with monad laws.
     finish honing.
   }
 
   apply reflexivityT.
-Defined.
+Admitted.
+
+End ByteStringHeap.
 
 End ByteStringHeap.
