src/Heap.v
@@ -6,7 +6,8 @@ Require Import
   ByteString.Memory
   ByteString.HeapState
   Coq.FSets.FMapFacts
-  Coq.Structures.DecidableTypeEx.
+  Coq.Structures.DecidableTypeEx
+  Hask.Control.Applicative.
 
 Module Heap (M : WSfun N_as_DT).
 
@@ -25,6 +26,19 @@ Definition pokeS    := "poke".
 Definition memcpyS  := "memcpy".
 Definition memsetS  := "memset".
 
+Section Heap.
+
+Context `{Alternative m}.
+
+Definition conditionally {rep A : Type} (r : rep)
+           (c : Comp (option A)) (Q : A -> Comp rep) : Comp (rep * m A) :=
+  mres <- c;
+  Ifopt mres as res
+  Then (r' <- Q res;
+        ret (r', pure res))
+  Else ret (r, empty).
+Arguments conditionally {rep A} r c Q _ /.
+
 Definition HeapSpec := Def ADT {
   (* Map of memory addresses to blocks, which contain another mapping from
      offsets to initialized bytes. *)
@@ -39,55 +53,62 @@ Definition HeapSpec := Def ADT {
      specify error handling at this level, when certain errors -- such as
      exhausting memory -- do not belong here, since a mathematical machine has
      no such limits. *)
-  Def Method1 allocS (r : rep) (len : Size | 0 < len) : rep * Ptr :=
-    addr <- find_free_block (` len) (resvs r);
-    ret ({| resvs := M.add addr (` len) (resvs r)
-          ; bytes := bytes r |}, addr),
+  Def Method1 allocS (r : rep) (len : Size | 0 < len) : rep * m Ptr :=
+    conditionally r (find_free_block (` len) (resvs r)) (fun addr =>
+      ret {| resvs := M.add addr (` len) (resvs r)
+           ; bytes := bytes r |}),
 
   (* Freeing an unallocated block is a no-op. *)
-  Def Method1 freeS (r : rep) (addr : Ptr) : rep * unit :=
-    ret ({| resvs := M.remove addr (resvs r)
-          ; bytes := bytes r |}, tt),
+  Def Method1 freeS (r : rep) (addr : Ptr) : rep * m unit :=
+    conditionally r { _ | True } (fun _ =>
+      ret {| resvs := M.remove addr (resvs r)
+           ; bytes := bytes r |}),
 
   (* Realloc is not required to reuse the same block. If the address does not
      identify an allociated region, a new memory block is returned without any
      bytes moved. If a block did exist previously, as many bytes as possible
      are copied to the new block. *)
   Def Method2 reallocS (r : rep) (addr : Ptr) (len : Size | 0 < len) :
-    rep * Ptr :=
-    naddr <- find_free_block (` len) (M.remove addr (resvs r));
-    ret ({| resvs := M.add naddr (` len) (M.remove addr (resvs r))
-          ; bytes :=
-              Ifopt M.find addr (resvs r) as sz
-              Then copy_bytes addr naddr (N.min sz (` len)) (bytes r)
-              Else bytes r |}, naddr),
+    rep * m Ptr :=
+    conditionally r (find_free_block (` len) (M.remove addr (resvs r)))
+      (fun naddr =>
+         ret {| resvs := M.add naddr (` len) (M.remove addr (resvs r))
+              ; bytes :=
+                  Ifopt M.find addr (resvs r) as sz
+                  Then copy_bytes addr naddr (N.min sz (` len)) (bytes r)
+                  Else bytes r |}),
 
   (* Peeking an uninitialized address allows any value to be returned. *)
-  Def Method1 peekS (r : rep) (addr : Ptr) : rep * Word :=
-    p <- { p : Word | forall v, M.MapsTo addr v (bytes r) -> p = v };
-    ret (r, p),
+  Def Method1 peekS (r : rep) (addr : Ptr) : rep * m Word :=
+    conditionally
+      r { p : option Word
+        | forall v, p = Some v -> M.MapsTo addr v (bytes r) }
+      (fun _ => ret r),
 
-  Def Method2 pokeS (r : rep) (addr : Ptr) (w : Word) : rep * unit :=
-    ret ({| resvs := resvs r
-          ; bytes := M.add addr w (bytes r) |}, tt),
+  Def Method2 pokeS (r : rep) (addr : Ptr) (w : Word) : rep * m unit :=
+    conditionally r { _ | True } (fun _ =>
+      ret {| resvs := resvs r
+           ; bytes := M.add addr w (bytes r) |}),
 
   (* Data may only be copied from one allocated block to another (or within
      the same block), and the region must fit within both source and
      destination. Otherwise, the operation is a no-op. *)
   Def Method3 memcpyS (r : rep) (addr1 : Ptr) (addr2 : Ptr) (len : Size) :
-    rep * unit :=
-    ret ({| resvs := resvs r
-          ; bytes := copy_bytes addr1 addr2 len (bytes r) |}, tt),
+    rep * m unit :=
+    conditionally r { _ | True } (fun _ =>
+      ret {| resvs := resvs r
+           ; bytes := copy_bytes addr1 addr2 len (bytes r) |}),
 
   (* Any attempt to memset bytes outside of an allocated block is a no-op. *)
   Def Method3 memsetS (r : rep) (addr : Ptr) (len : Size) (w : Word) :
-    rep * unit :=
-    ret ({| resvs := resvs r
-          ; bytes :=
-              P.update (bytes r)
-                       (N.peano_rect (fun _ => M.t Word) (bytes r)
-                                     (fun i => M.add (addr + i)%N w)
-                                     len) |}, tt)
+    rep * m unit :=
+    conditionally r { _ | True } (fun _ =>
+      ret {| resvs := resvs r
+           ; bytes :=
+               P.update (bytes r)
+                        (N.peano_rect (fun _ => M.t Word) (bytes r)
+                                      (fun i => M.add (addr + i)%N w)
+                                      len) |})
 
 }%ADTParsing.
 
@@ -95,31 +116,31 @@ Definition empty : Comp (Rep HeapSpec) :=
   Eval simpl in callCons HeapSpec emptyS.
 
 Definition alloc (r : Rep HeapSpec) (len : Size | 0 < len) :
-  Comp (Rep HeapSpec * N) :=
+  Comp (Rep HeapSpec * m N) :=
   Eval simpl in callMeth HeapSpec allocS r len.
 
 Definition free (r : Rep HeapSpec) (addr : Ptr) :
-  Comp (Rep HeapSpec * unit) :=
+  Comp (Rep HeapSpec * m unit) :=
   Eval simpl in callMeth HeapSpec freeS r addr.
 
 Definition realloc (r : Rep HeapSpec) (addr : Ptr) (len : Size | 0 < len) :
-  Comp (Rep HeapSpec * N) :=
+  Comp (Rep HeapSpec * m N) :=
   Eval simpl in callMeth HeapSpec reallocS r addr len.
 
 Definition peek (r : Rep HeapSpec) (addr : Ptr) :
-  Comp (Rep HeapSpec * Word) :=
+  Comp (Rep HeapSpec * m Word) :=
   Eval simpl in callMeth HeapSpec peekS r addr.
 
 Definition poke (r : Rep HeapSpec) (addr : Ptr) (w : Word) :
-  Comp (Rep HeapSpec * unit) :=
+  Comp (Rep HeapSpec * m unit) :=
   Eval simpl in callMeth HeapSpec pokeS r addr w.
 
 Definition memcpy (r : Rep HeapSpec) (addr : Ptr) (addr2 : Ptr) (len : Size) :
-  Comp (Rep HeapSpec * unit) :=
+  Comp (Rep HeapSpec * m unit) :=
   Eval simpl in callMeth HeapSpec memcpyS r addr addr2 len.
 
 Definition memset (r : Rep HeapSpec) (addr : Ptr) (len : Ptr) (w : Word) :
-  Comp (Rep HeapSpec * unit) :=
+  Comp (Rep HeapSpec * m unit) :=
   Eval simpl in callMeth HeapSpec memsetS r addr len w.
 
 (**
@@ -131,10 +152,11 @@ Ltac inspect :=
   repeat breakdown;
   repeat (simplify_maps; simpl in *;
           destruct_computations; simpl in *;
-          repeat breakdown).
+          repeat breakdown);
+  simpl in *; tsubst; simpl in *.
 
 Ltac complete IHfromADT :=
-  inspect;
+  repeat inspect;
   try match goal with
     [ H : (?X =? ?Y) = true |- _ ] => apply N.eqb_eq in H; subst
   end;
@@ -144,6 +166,8 @@ Ltac complete IHfromADT :=
             | inspect; try nomega;
               eapply IHfromADT; try eassumption; inspect
             | discriminate ].
+
+(* Typeclasses eauto := debug. *)
 
 Theorem allocations_have_size : forall r : Rep HeapSpec, fromADT _ r ->
   forall addr sz, M.MapsTo addr sz (resvs r) -> 0 < sz.
@@ -161,8 +185,8 @@ Theorem allocations_no_overlap : forall r : Rep HeapSpec, fromADT _ r ->
     -> ~ overlaps addr1 sz1 addr2 sz2.
 Proof.
   intros.
-  pose proof (allocations_have_size H H0).
-  pose proof (allocations_have_size H H1).
+  pose proof (allocations_have_size H0 H1).
+  pose proof (allocations_have_size H0 H2).
   generalize dependent sz2.
   generalize dependent addr2.
   generalize dependent sz1.
@@ -170,10 +194,10 @@ Proof.
   ADT induction r; complete IHfromADT.
   - apply_for_all; nomega.
   - apply_for_all; nomega.
-  - eapply M.remove_2 in H4; eauto.
+  - eapply M.remove_2 in H5; eauto.
     apply_for_all; nomega.
-  - clear H8.
-    eapply M.remove_2 in H4; eauto.
+  - clear H9.
+    eapply M.remove_2 in H5; eauto.
     apply not_overlaps_sym.
     apply_for_all; nomega.
 Qed.
@@ -188,49 +212,49 @@ Proof.
   generalize dependent sz1.
   generalize dependent addr1.
   ADT induction r; complete IHfromADT.
-  - inversion H2.
+  - inversion H3.
     simplify_maps.
-  - apply (proj1 (in_mapsto_iff _ _ _)) in H2.
-    destruct H2.
-    apply for_all_add_true in H1;
+  - apply (proj1 (in_mapsto_iff _ _ _)) in H3.
+    destruct H3.
+    apply for_all_add_true in H2;
     relational; simpl in *.
       simplify_maps.
         nomega.
       assert (M.In addr1 (resvs r)).
         apply in_mapsto_iff.
-        exists x1; assumption.
+        exists x0; assumption.
       eapply IHfromADT; eauto.
       nomega.
     unfold not; intros.
     eapply IHfromADT; eauto.
-  - apply (proj1 (in_mapsto_iff _ _ _)) in H2.
-    destruct H2.
+  - apply (proj1 (in_mapsto_iff _ _ _)) in H3.
+    destruct H3.
     simplify_maps.
-    eapply for_all_remove_inv in H1; relational.
+    eapply for_all_remove_inv in H2; relational.
       eapply IHfromADT; eauto.
       apply in_mapsto_iff.
       exists x0; assumption.
     unfold not; intros.
-    apply (proj1 (in_mapsto_iff _ _ _)) in H0.
-    destruct H0.
-    pose proof (allocations_have_size H H4).
-    apply not_eq_sym in H2.
-    eapply F.remove_neq_mapsto_iff in H4; eauto.
+    apply (proj1 (in_mapsto_iff _ _ _)) in H3.
+    destruct H3.
+    pose proof (allocations_have_size H0 H6).
+    apply not_eq_sym in H5.
+    eapply F.remove_neq_mapsto_iff in H6; eauto.
     apply_for_all; relational.
     nomega.
-  - apply (proj1 (in_mapsto_iff _ _ _)) in H2.
-    destruct H2.
+  - apply (proj1 (in_mapsto_iff _ _ _)) in H3.
+    destruct H3.
     simpl in *.
     apply_for_all; relational.
-    rewrite <- remove_add in H1.
+    rewrite <- remove_add in H2.
     simplify_maps.
-      apply for_all_add_true in H1; relational; simpl in *.
+      apply for_all_add_true in H2; relational; simpl in *.
         nomega.
       simplify_maps.
-    rewrite remove_add in H1.
+    rewrite remove_add in H2.
     apply_for_all; relational.
     simplify_maps.
-    pose proof (allocations_have_size H H6).
+    pose proof (allocations_have_size H0 H7).
     nomega.
 Qed.
 
@@ -242,11 +266,13 @@ Corollary allocations_no_overlap_for_all :
                 (M.remove addr (resvs r)).
 Proof.
   intros.
-  pose proof (allocations_no_overlap H H0).
+  pose proof (allocations_no_overlap H0 H1).
   apply P.for_all_iff; relational; intros.
   simplify_maps.
-  specialize (H1 _ _ H4 H3).
+  specialize (H2 _ _ H5 H4).
   nomega.
 Qed.
+
+End Heap.
 
 End Heap.
