lib/Option.v
@@ -1,0 +1,102 @@
+Require Import Hask.Control.Monad.
+
+Generalizable All Variables.
+
+Notation Maybe   := option.
+Notation Nothing := None.
+Notation Just    := Some.
+
+Definition fromoption `(x : a) (my : option a) : a :=
+  match my with
+ | Just z  => z
+ | Nothing => x
+  end.
+
+Definition fold_option `(x : b) `(f : a -> b) (my : option a) : b :=
+  match my with
+ | Just z  => f z
+ | Nothing => x
+  end.
+
+Definition option_map `(f : X -> Y) (x : option X) : option Y :=
+  match x with
+  | Nothing => Nothing
+  | Just x' => Just (f x')
+  end.
+
+Instance option_Functor : Functor option :=
+{ fmap := @option_map
+}.
+
+Definition option_apply {X Y} (f : option (X -> Y)) (x : option X) : option Y :=
+  match f with
+  | Nothing => Nothing
+  | Just f' => match x with
+    | Nothing => Nothing
+    | Just x' => Just (f' x')
+    end
+  end.
+
+Instance option_Applicative : Applicative option :=
+{ is_functor := option_Functor
+; pure := @Just
+; ap := @option_apply
+}.
+
+Definition option_join {X} (x : option (option X)) : option X :=
+  match x with
+  | Nothing => Nothing
+  | Just Nothing => Nothing
+  | Just (Just x') => Just x'
+  end.
+
+Instance option_Monad : Monad option :=
+{ is_applicative := option_Applicative
+; join := @option_join
+}.
+
+(* jww (2015-06-17): NYI
+Ltac simple_solver :=
+  intros;
+  try extensionality e;
+  compute;
+  repeat (
+    match goal with
+    | [ |- context f [match ?X with _ => _ end] ] =>
+      is_var X; destruct X; auto
+    end);
+  auto.
+
+(** By registering our simple_solver as the obligation tactic, all our law
+    obligations will be taken care of for us automatically by the Ltac
+    scripts above. *)
+Obligation Tactic := simple_solver.
+*)
+
+Definition isJust {a} (x : option a) := if x then true else false.
+
+Definition option_choose {a} (x y : option a) : option a :=
+  match x with
+  | Nothing => y
+  | Just _  => x
+  end.
+
+Instance option_Alternative : Alternative option := {
+  empty  := @Nothing;
+  choose := @option_choose
+  (* some := fun _ x => match x with *)
+  (*   | Nothing => Nothing *)
+  (*   | Just x => Just [x] *)
+  (*   end; *)
+  (* many := fun _ x => match x with *)
+  (*   | Nothing => Just [] *)
+  (*   | Just x => [x] *)
+  (*   end *)
+}.
+
+Lemma option_choose_spec : forall a (x y : option a),
+  isJust (x <|> y) = (isJust x || isJust y)%bool.
+Proof.
+  intros a x y.
+  destruct x; auto.
+Qed.
